src/Distributions/Uniform/Correctness.dfy
@@ -99,26 +99,13 @@ module Uniform.Correctness {
     UniformPowerOfTwo.Correctness.UnifCorrectness2(2 * n, i);
   }
 
-  lemma Power2Log2Helper(n: nat)
-    requires n >= 1
-    ensures n < Helper.Power(2, Helper.Log2Floor(2 * n))
-  {
-    calc {
-      n;
-    < { Helper.Power2OfLog2Floor(n); }
-      Helper.Power(2, Helper.Log2Floor(n) + 1);
-    == { Helper.Log2FloorDef(n); }
-      Helper.Power(2, Helper.Log2Floor(2 * n));
-    }
-  }
-
   lemma ProbabilityProposalAccepted(n: nat)
     requires n >= 1
     ensures
       RandomNumberGenerator.mu(WhileAndUntil.ProposalAcceptedEvent(Model.Proposal(n), Model.Accept(n))) == (n as real) / (Helper.Power(2, Helper.Log2Floor(2 * n)) as real)
   {
     var e := WhileAndUntil.ProposalAcceptedEvent(Model.Proposal(n), Model.Accept(n));
-    assert n < Helper.Power(2, Helper.Log2Floor(2 * n)) by { Power2Log2Helper(n); }
+    assert n < Helper.Power(2, Helper.Log2Floor(2 * n)) by { Helper.NLtPower2Log2FloorOf2N(n); }
     assert Equal: e == (iset s | UniformPowerOfTwo.Model.Sample(2 * n)(s).0 < n) by {
       forall s ensures s in e <==> UniformPowerOfTwo.Model.Sample(2 * n)(s).0 < n {
         calc {
@@ -162,7 +149,16 @@ module Uniform.Correctness {
   }
 
   // Equation (4.10)
-  lemma {:axiom} SampleIsIndepFn(n: nat)
+  lemma SampleIsIndepFn(n: nat)
     requires n > 0
     ensures Independence.IsIndepFn(Model.Sample(n))
+  {
+    assert Independence.IsIndepFn(Model.Proposal(n)) by {
+      UniformPowerOfTwo.Correctness.SampleIsIndepFn(2 * n);
+    }
+    assert WhileAndUntil.ProbUntilTerminates(Model.Proposal(n), Model.Accept(n)) by {
+      Model.SampleTerminates(n);
+    }
+    WhileAndUntil.ProbUntilIsIndepFn(Model.Proposal(n), Model.Accept(n));
+  }
 }
